Change qsort to use proven in-bounds accesses

src/Init/Data/Array/QSort.lean
@@ -7,41 +7,131 @@ prelude
 import Init.Data.Array.Basic
 
 namespace Array
--- TODO: remove the [Inhabited α] parameters as soon as we have the tactic framework for automating proof generation and using Array.fget
 
 def qpartition (as : Array α) (lt : α → α → Bool) (lo hi : Nat) : Nat × Array α :=
-  if h : as.size = 0 then (0, as) else have : Inhabited α := ⟨as[0]'(by revert h; cases as.size <;> simp)⟩ -- TODO: remove
-  let mid := (lo + hi) / 2
-  let as  := if lt (as.get! mid) (as.get! lo) then as.swap! lo mid else as
-  let as  := if lt (as.get! hi)  (as.get! lo) then as.swap! lo hi  else as
-  let as  := if lt (as.get! mid) (as.get! hi) then as.swap! mid hi else as
-  let pivot := as.get! hi
-  let rec loop (as : Array α) (i j : Nat) :=
-    if h : j < hi then
-      if lt (as.get! j) pivot then
-        let as := as.swap! i j
-        loop as (i+1) (j+1)
-      else
-        loop as i (j+1)
-    else
-      let as := as.swap! i hi
-      (i, as)
-    termination_by hi - j
-    decreasing_by all_goals simp_wf; decreasing_trivial_pre_omega
-  loop as lo lo
+  let s := as.size
+  have hs: as.size = s := rfl
 
-@[inline] partial def qsort (as : Array α) (lt : α → α → Bool) (low := 0) (high := as.size - 1) : Array α :=
+  let hi := if hi < s then hi else s - 1
+
+  if hlh: lo ≥ hi then (lo, as) else
+  have hlh: lo < hi := Nat.gt_of_not_le hlh
+
+  have h0s: s ≠ 0 := by
+    dsimp only [hi] at hlh
+    split at hlh
+    case isTrue h =>
+      exact Nat.not_eq_zero_of_lt h
+    case isFalse h =>
+      apply Nat.ne_of_gt
+      apply Nat.zero_lt_of_lt
+      exact Nat.add_lt_of_lt_sub hlh
+
+  have hhs: hi < s := by
+    dsimp only [hi]
+    split
+    · assumption
+    · apply Nat.sub_one_lt
+      exact h0s
+
+  -- we need this since otherwise loop doesn't capture hi, but rather what it unfolds to
+  have ⟨hi, hlh, hhs⟩: (hi: Nat) ×' (lo < hi) ×' (hi < s) := ⟨hi, hlh, hhs⟩
+
+  have hls: lo < s := Nat.lt_trans hlh hhs
+
+  let mid := (lo + hi) / 2
+
+  have hms: mid < s := by
+    apply Nat.div_lt_of_lt_mul
+    rw [Nat.two_mul]
+    exact Nat.add_lt_add hls hhs
+
+  let b := lt as[mid] as[lo]
+  let as := if b then as.swap ⟨lo, hs ▸ hls⟩ ⟨mid, hs ▸ hms⟩ else as
+  have hs: as.size = s := by dsimp only [as]; split; all_goals simp_all only [Array.size_swap]
+
+  -- we need let b since otherwise the split tactic fails
+  let b := lt as[hi] as[lo]
+  let as  := if b then as.swap ⟨lo, hs ▸ hls⟩ ⟨hi, hs ▸ hhs⟩  else as
+  have hs: as.size = s := by dsimp only [as]; split; all_goals simp_all only [Array.size_swap]
+
+  let b := lt as[mid] as[hi]
+  let as := if b then as.swap ⟨mid, hs ▸ hms⟩ ⟨hi, hs ▸ hhs⟩ else as
+  have hs: as.size = s := by dsimp only [as]; split; all_goals simp_all only [Array.size_swap]
+
+  let pivot := as[hi]
+
+  let rec loop (as : Array α) (i j : Nat) (hij: i ≤ j) (hjh: j ≤ hi) (hhs: hi < as.size):=
+    let s := as.size
+    have hs: as.size = s := rfl
+
+    have his: i < s := Nat.lt_of_le_of_lt hij (Nat.lt_of_le_of_lt hjh hhs)
+
+    if hjh : j < hi then
+      have hjs: j < s := Nat.lt_trans hjh hhs
+
+      if lt as[j] pivot then
+        let as := as.swap ⟨i, hs ▸ his⟩ ⟨j, hs ▸ hjs⟩
+        have hs: as.size = s := by simp_all only [as, Array.size_swap]
+
+        have hij: i + 1 ≤ j + 1 := Nat.add_le_add_right hij 1
+
+        loop as (i+1) (j+1) hij hjh (hs ▸ hhs)
+      else
+        have hij: i ≤ j + 1 := Nat.le_add_right_of_le hij
+
+        loop as i (j+1) hij hjh (hs ▸ hhs)
+    else
+      let as := as.swap ⟨i, hs ▸ his⟩ ⟨hi, hs ▸ hhs⟩
+      (i, as)
+
+  have hlh: lo ≤ hi := Nat.le_of_succ_le hlh
+  have hll: lo ≤ lo := Nat.le_refl lo
+
+  loop as lo lo hll hlh (hs ▸ hhs)
+
+theorem i_le_qpartition_loop_fst (lt: α → α → Bool) {hi: Nat} (pivot: α) {as: Array α} {i: Nat} {j: Nat}
+    (hij: i ≤ j) (hjh: j ≤ hi) (hhs: hi < as.size):
+  i ≤ (qpartition.loop lt hi pivot as i j hij hjh hhs).1 := by
+  unfold qpartition.loop
+  -- the split tactic fails
+  by_cases hjh: j < hi
+  all_goals simp only [hjh, ↓reduceDIte]
+  · split
+    · apply Nat.le_of_succ_le
+      apply i_le_qpartition_loop_fst
+    · apply i_le_qpartition_loop_fst
+  · apply Nat.le_refl
+
+theorem lo_le_qpartition_fst (as: Array α) (lt: α → α → Bool) (lo hi: Nat):
+    lo ≤ (qpartition as lt lo hi).1 := by
+  unfold qpartition
+  -- the split tactic fails
+  by_cases hlh: lo ≥ (if hi < as.size then hi else as.size - 1)
+  all_goals simp only [hlh, ↓reduceDIte]
+  · apply Nat.le_refl
+  · apply i_le_qpartition_loop_fst
+
+@[inline] def qsort (as : Array α) (lt : α → α → Bool) (low := 0) (high := as.size - 1) : Array α :=
   let rec @[specialize] sort (as : Array α) (low high : Nat) :=
-    if low < high then
-      let p := qpartition as lt low high;
-      -- TODO: fix `partial` support in the equation compiler, it breaks if we use `let (mid, as) := partition as lt low high`
+    if hlh: low < high then
+      let p := qpartition as lt low high
       let mid := p.1
       let as  := p.2
-      if mid >= high then as
+      if hmh: mid >= high then as
       else
         let as := sort as low mid
         sort as (mid+1) high
     else as
-  sort as low high
+  termination_by high - low
+  decreasing_by
+    · apply Nat.sub_lt_sub_right
+      · apply lo_le_qpartition_fst
+      · exact Nat.gt_of_not_le hmh
+    · apply Nat.sub_lt_sub_left
+      · exact hlh
+      · apply Nat.lt_succ_of_le
+        apply lo_le_qpartition_fst
 
+  sort as low high
 end Array
